cleaned

basic_types.v
@@ -1,9 +1,9 @@
+(*Trivial facts that would clutter up the other files*)
 Require Import ssreflect.
 From mathcomp Require Import ssreflect seq ssrnat.
 From istari Require Import Sigma Tactics
      Syntax Subst SimpSub Promote Hygiene
-     ContextHygiene Equivalence.
-From istari Require Import Rules Defined.
+     ContextHygiene Equivalence Rules Defined.
 
 Definition oof M A: (@Syntax.judgement False) := deq M M A.
 
@@ -13,6 +13,9 @@ Definition U0 : (term False) := univ nzero.
 
 Definition leq_t n m : term False :=
   app (app leqtp n) m.
+
+Definition lt_t n m : term False :=
+  app (app lttp n) m.
 
 Lemma zero_typed: forall G,
     tr G (oof nzero nattp). Admitted.
@@ -32,8 +35,12 @@ Lemma lt_type: forall G n1 n2,
     tr G (oof (ltpagetp n1 n2) U0).
   Admitted.
 
-Hint Resolve zero_typed.
-Hint Resolve leq_refl.
-Hint Resolve leq_type.
-Hint Resolve lt_type.
+Lemma nat_U0: forall G,
+    tr G (oof nattp U0). Admitted.
+
+Lemma nat_type: forall G,
+      tr G (deqtype nattp nattp). Admitted.
+
+Hint Resolve nat_type nat_U0 zero_typed leq_refl leq_type lt_type.
+
 
