derived_rules.v
@@ -1,0 +1,90 @@
+Require Import Program.Equality Ring Lia Omega.
+From mathcomp Require Import ssreflect ssrfun ssrbool seq eqtype ssrnat.
+From istari Require Import source subst_src rules_src help subst_help trans basic_types.
+From istari Require Import Sigma Tactics
+     Syntax Subst SimpSub Promote Hygiene
+     ContextHygiene Equivalence Rules Defined.
+
+(*more useful inference rules*)
+
+Lemma tr_arrow_elim: forall G a b m n p q,
+    tr G (deqtype a a) ->
+    tr G (deqtype b b) ->
+      tr G (deq m n (arrow a b))
+      -> tr G (deq p q a) 
+      -> tr G (deq (app m p) (app n q) b).
+intros. 
+suffices: (subst1 p (subst sh1 b)) = b. move => Heq.
+rewrite - Heq.
+eapply (tr_pi_elim _ a); try assumption.
+eapply tr_eqtype_convert; try apply tr_arrow_pi_equal; assumption.
+simpsub. auto. Qed.
+
+Lemma tr_arrow_intro: forall G a b m n,
+    tr G (deqtype a a) ->
+      tr G (deqtype b b)
+      -> tr (cons (hyp_tm a) G) (deq m n (subst sh1 b))
+      -> tr G (deq (lam m) (lam n) (arrow a b) ).
+intros. eapply tr_eqtype_convert.
+apply tr_eqtype_symmetry. apply tr_arrow_pi_equal; try assumption.
+eapply tr_pi_intro; try assumption. Qed.
+
+Lemma tr_karrow_elim: forall G a b m n p q,
+    tr G (deqtype a a) ->
+    tr G (deqtype b b) ->
+      tr G (deq m n (karrow a b))
+      -> tr G (deq p q a) 
+      -> tr G (deq (app m p) (app n q) b).
+  intros. apply (tr_arrow_elim _ a); try assumption.
+  eapply tr_eqtype_convert. apply tr_eqtype_symmetry.
+  apply tr_arrow_karrow_equal; assumption.
+  assumption. Qed.
+
+Lemma kind_type: forall {G K i},
+    tr G (deq K K (kuniv i)) -> tr G (deqtype K K).
+  intros. eapply tr_formation_weaken.
+  eapply tr_kuniv_weaken. apply X. Qed.
+
+Lemma nat_U0: forall G,
+    tr G (oof nattp U0). Admitted.
+Hint Resolve nat_U0. 
+
+Lemma nat_type: forall G,
+      tr G (deqtype nattp nattp). Admitted.
+Hint Resolve nat_type. 
+
+Lemma tr_weakening_appends: forall G1 G2 G3 J1 J2 t J1' J2' t',
+    tr G1 (deq J1 J2 t) ->
+    J1' = (shift (size G2) J1) ->
+    J2' = (shift (size G2) J2) ->
+    t' = (shift (size G2) t) ->
+    G3 = G2 ++ G1 ->
+      tr G3 (deq J1' J2' t').
+ intros. move: G3 t t' J1' J2' J1 J2 H H0 H1 H2 X. induction G2; intros.
+ -  simpl. subst. repeat rewrite - subst_sh_shift. simpsub. assumption.
+ -
+  suffices: (tr (substctx sh1 [::] ++ cons a (G2 ++ G1))
+                (substj (under (length [::]) sh1)
+                        (substj (sh (size G2)) (deq J1 J2 t)))).
+  move => Hdone.
+  simpl in Hdone. subst.
+  rewrite (size_ncons 1).
+  rewrite - plusE. 
+  repeat rewrite subst_sh_shift.
+  repeat rewrite - shift_sum.
+  repeat rewrite subst_sh_shift in Hdone.
+  rewrite cat_cons.
+ apply (Hdone False). 
+ intros.
+ eapply tr_weakening.
+ simpl. repeat rewrite subst_sh_shift. eapply IHG2; try reflexivity. assumption.
+Qed.
+
+ Lemma tr_weakening_append: forall (G1: context) G2 J1 J2 t,
+      tr G1 (deq J1 J2 t) ->
+      tr (G2 ++ G1) (
+                       (deq (shift (size G2) J1)
+                            (shift (size G2) J2)
+                            (shift (size G2) t))).
+   intros. eapply tr_weakening_appends; try apply X; try reflexivity.
+   Qed.
