embedded_lemmas.v
@@ -1,0 +1,295 @@
+Require Import Program.Equality Ring Lia Omega.
+From mathcomp Require Import ssreflect ssrfun ssrbool seq eqtype ssrnat.
+From istari Require Import source subst_src rules_src help subst_help0 subst_help
+     trans basic_types derived_rules.
+From istari Require Import Sigma Tactics
+     Syntax Subst SimpSub Promote Hygiene
+     ContextHygiene Equivalence Rules Defined.
+(*useful properties of the embedding*)
+
+Ltac var_solv :=
+  try (apply tr_hyp_tm; repeat constructor).
+
+(*quick facts about worlds*)
+
+(*preworlds can indeed be impredicatively quantified over *)
+Lemma pw_kind: forall {G},
+    tr G (deq preworld preworld (kuniv nzero)).
+  intros. apply tr_rec_kind_formation.
+  apply tr_arrow_kind_formation.
+  auto. apply tr_karrow_kind_formation.
+  apply tr_fut_kind_formation.
+  simpl. rewrite - subst_kuniv.
+  apply tr_hyp_tm. repeat constructor.
+  auto.
+  apply tr_arrow_kind_formation. apply tr_fut_formation_univ.
+  rewrite subst_nzero. apply nat_U0. auto.
+  apply tr_univ_kind_formation; auto. apply zero_typed. Qed.
+
+Lemma pw_type: forall {G},
+    tr G (deqtype preworld preworld ).
+  intros. apply (kind_type pw_kind). Qed.
+
+Hint Resolve pw_kind pw_type.
+
+(*subtypes of preworld*)
+Lemma pw_type2: forall {G}, tr G (deqtype (arrow (fut nattp) (univ nzero))
+                                   (arrow (fut nattp) (univ nzero))).
+  intros. apply tr_arrow_formation.
+  apply tr_fut_formation. auto.
+  apply tr_univ_formation. auto. Qed.
+
+Lemma pw_type1: forall {G}, tr G (deqtype
+       (karrow (fut preworld) (arrow (fut nattp) (univ nzero)))
+       (karrow (fut preworld) (arrow (fut nattp) (univ nzero)))
+  ).
+  intros. apply tr_karrow_formation.
+  apply tr_fut_formation. auto. apply pw_type2. Qed.
+
+
+Lemma unfold_pw: forall G,
+    tr G (deqtype preworld (arrow nattp
+          (karrow (fut preworld) (arrow (fut nattp) (univ nzero))))). Admitted.
+
+Lemma split_world_elim2: forall W G,
+    tr G (oof W world) -> tr G (oof (ppi2 W) nattp).
+Admitted.
+
+Lemma split_world_elim1: forall W G,
+    tr G (oof W world) -> tr G (oof (ppi1 W) preworld).
+Admitted.
+
+Lemma world_type: forall G,
+      tr G (deqtype world world). Admitted.
+Hint Resolve world_type. 
+
+    Lemma split_world1: forall w1 l1 G,
+tr G (oof (ppair w1 l1) world) -> tr G (oof w1 preworld). (*ask karl can't put a
+                                                          conjunction here*)
+    Admitted.
+
+    Lemma split_world2: forall w1 l1 G,
+tr G (oof (ppair w1 l1) world) -> tr G (oof l1 nattp). (*ask karl can't put a
+                                                          conjunction here*)
+    Admitted.
+
+    Lemma nth_works: forall G w n,
+        tr G (oof w world) -> tr G (oof n nattp) -> tr G (oof (nth w n)
+                           (karrow (fut preworld) (arrow (fut nattp) U0))).
+      intros. unfold nth. apply (tr_arrow_elim _ nattp); auto.
+      do 2? constructor. auto.
+      constructor. auto.
+      apply tr_univ_formation. auto.
+      eapply tr_eqtype_convert. apply unfold_pw.
+      apply split_world_elim1. assumption.
+      Qed.
+
+(*longer facts about worlds*)
+Lemma subseq_U0: forall G w1 w2,
+    tr G (oof w1 world) -> tr G (oof w2 world) ->
+    tr G (oof (subseq w1 w2) (univ nzero)).
+  intros.
+  assert (forall V,
+tr [:: hyp_tm
+          (leq_t (var 0)
+             (subst (sh 3) (ppi2 (var 0)))),
+        hyp_tm nattp, hyp_tm (fut nattp),
+        hyp_tm (fut preworld), hyp_tm world,
+        hyp_tm world
+        & G] (oof V world) ->
+
+  tr
+    [:: hyp_tm
+          (leq_t (var 0)
+             (subst (sh 3) (ppi2 (var 0)))),
+        hyp_tm nattp, hyp_tm (fut nattp),
+        hyp_tm (fut preworld), hyp_tm world,
+        hyp_tm world
+      & G]
+    (oof
+       (app3 (ppi1 V) 
+          (var 1) (var 3) (var 2)) 
+     (univ nzero))
+         ) as Hworldapp.
+  intros V Hvw.
+
+  rewrite - (subst_nzero (dot (var 2) id)). (*start of the application proof,
+                                              make this general for any
+                                              (var 0) which gamma says is world*)
+  rewrite - subst_univ.
+  eapply (tr_pi_elim _ (fut nattp) ).
+   simpsub. simpl.
+  assert (forall s, pi (fut nattp) (univ nzero)
+                     =  @subst False s (pi (fut nattp) (univ nzero))
+         ) as sub1.
+  auto.
+  assert (forall s, @subst False s (karrow (fut preworld) (arrow (fut nattp) (univ nzero)))
+                     = (karrow (fut preworld) (arrow (fut nattp) (univ nzero)))
+         ) as sub2.
+  auto.
+  assert (forall s, arrow (fut nattp) (univ nzero)
+                     =  @subst False s (arrow (fut nattp) (univ nzero))
+         ) as sub3.
+  auto.
+  eapply tr_eqtype_convert.
+  rewrite - (subst_U0 (sh 1)).
+  eapply tr_arrow_pi_equal.
+  eapply tr_fut_formation. eapply nat_type.
+  eapply tr_univ_formation.
+  apply zero_typed.
+  rewrite (sub3 (dot (var 3) id)).
+  eapply (tr_pi_elim _ (fut preworld)).
+  eapply tr_eqtype_convert.
+  rewrite (sub3 sh1).
+  eapply tr_arrow_pi_equal.
+  eapply tr_fut_formation. eapply pw_type.
+  eapply pw_type2.
+  assert (forall s, (arrow (fut preworld)
+          (arrow (fut nattp) (univ nzero)))
+               =  @subst False s (arrow (fut preworld)
+          (arrow (fut nattp) (univ nzero)))
+)
+    as sub4.
+  auto.
+  eapply tr_eqtype_convert.
+  eapply tr_eqtype_symmetry.
+  eapply tr_arrow_karrow_equal.
+  eapply tr_fut_formation. eapply pw_type.
+  eapply pw_type2.
+  rewrite - (sub2 (dot (var 1) id)).
+  eapply (tr_pi_elim _ nattp).
+  eapply tr_eqtype_convert.
+  rewrite - (sub2 (sh1)).
+  eapply tr_arrow_pi_equal.
+  apply nat_type.
+  eapply pw_type1.
+  eapply tr_eqtype_convert.
+  apply unfold_pw.
+  eapply (tr_sigma_elim1 _ _ nattp).
+  (*assert (forall s, (arrow nattp
+             (karrow (fut preworld) (arrow (fut nattp) (univ nzero))))
+               =  @subst False s (arrow nattp
+             (karrow (fut preworld) (arrow (fut nattp) (univ nzero))))
+)
+    as sub5.
+  intros. auto.*)
+  apply Hvw.
+  (*assert (sigma preworld nattp = world) by auto. rewrite H.
+  rewrite - {3}(subst_world (sh 5)).
+  apply tr_hyp_tm. repeat constructor.*)
+  rewrite - {3}(subst_nat (sh 2)).
+  apply tr_hyp_tm. repeat constructor.
+  rewrite - {2}(subst_pw (sh 4)).
+  rewrite - subst_fut.
+  apply tr_hyp_tm. repeat constructor.
+  rewrite - {2}(subst_nat (sh 3)).
+  rewrite - subst_fut.
+  apply tr_hyp_tm. repeat constructor.
+  simpsub. simpl.
+
+
+unfold subseq.
+  rewrite - (subst_nzero (dot w2 id)).
+  rewrite - subst_univ.
+  eapply (tr_pi_elim _ world).
+  rewrite - (subst_nzero (under 1 (dot w1 id)) ).
+  rewrite - subst_univ.
+  rewrite - (subst_world (dot w1 id)).
+  rewrite - subst_pi.
+  eapply (tr_pi_elim _ world).
+  apply tr_pi_intro. apply world_type.
+  apply tr_pi_intro. apply world_type.
+  eapply tr_prod_formation_univ.
+  eapply leq_type.
+  eapply split_world_elim2.
+  rewrite - (subst_world (sh 1)).
+  eapply tr_hyp_tm. constructor.
+  eapply split_world_elim2.
+  rewrite - (subst_world (sh 2)).
+  eapply tr_hyp_tm. repeat constructor.
+  eapply tr_all_formation_univ.
+  eapply tr_fut_kind_formation.
+  apply pw_kind.
+  apply zero_typed.
+  eapply tr_pi_formation_univ.
+  eapply tr_fut_formation_univ.
+  apply nat_U0.
+  repeat rewrite subst_nzero. apply zero_typed.
+  repeat rewrite subst_nzero.
+  eapply tr_pi_formation_univ. apply nat_U0.
+  repeat rewrite subst_nzero. eapply tr_pi_formation_univ.
+  apply leq_type.
+  rewrite - (subst_nat (sh 1)).
+  eapply tr_hyp_tm. repeat constructor.
+  rewrite subst_ppi2. simpsub. simpl.
+  eapply split_world_elim2.
+  rewrite - (subst_world (sh 4)).
+  eapply tr_hyp_tm. repeat constructor.
+  repeat rewrite subst_nzero.
+  eapply tr_eqtype_formation_univ.
+apply Hworldapp. 
+  rewrite - {3}(subst_world (sh 5)).
+  apply tr_hyp_tm. repeat constructor.
+simpsub. simpl. apply Hworldapp. 
+  rewrite - {3}(subst_world (sh 6)).
+  apply tr_hyp_tm. repeat constructor.
+  auto.
+  repeat rewrite subst_nzero. apply leq_refl. auto.
+assumption. assumption.
+Qed.
+
+(*simple lemmas about well typedness of embedding*)
+Lemma laters_type: forall A G i,
+    (tr G (oof A (univ i))) -> tr G (oof (laters A) (univ i)).
+  Admitted.
+Hint Resolve laters_type.
+
+Lemma bind_type: forall G A B M0 M1,
+    tr G (oof M0 (laters A)) ->
+    tr G (oof M1 (arrow A (laters B))) ->
+    tr G (oof (make_bind M0 M1) (laters B)). Admitted.
+
+(*repeated patterns of proofs.v*)
+
+Lemma world_pair: forall w l G, tr G (oof w preworld) ->
+                           tr G (oof l nattp) ->
+    tr G (oof (ppair w l) world).
+  intros. eapply tr_sigma_intro; try assumption.
+  apply nat_type. Qed.
+
+Lemma uworld10: forall G,
+      (tr [:: hyp_tm nattp, hyp_tm preworld & G]
+    (oof (ppair (var 1) (var 0)) world)). intros.
+     apply world_pair. 
+        rewrite - (subst_pw (sh 2)).
+      apply tr_hyp_tm; repeat constructor.
+        rewrite - (subst_nat (sh 1)).
+        apply tr_hyp_tm; repeat constructor. Admitted.
+
+Lemma uworld21: forall G x,
+      (tr [:: x, hyp_tm nattp, hyp_tm preworld & G]
+    (oof (ppair (var 2) (var 1)) world)). intros.
+   apply world_pair.
+  rewrite - (subst_pw (sh 3)). var_solv.
+  rewrite - (subst_nat (sh 2)). var_solv. Qed. 
+
+Lemma uworld32: forall G x y,
+      (tr [:: x, y, hyp_tm nattp, hyp_tm preworld & G]
+    (oof (ppair (var 3) (var 2)) world)). intros.
+   apply world_pair.
+  rewrite - (subst_pw (sh 4)). var_solv.
+  rewrite - (subst_nat (sh 3)). var_solv. Qed. 
+
+  Lemma uworld43: forall G x y z,
+      (tr [:: x, y, z, hyp_tm nattp, hyp_tm preworld & G]
+    (oof (ppair (var 4) (var 3)) world)). intros.
+   apply world_pair.
+  rewrite - (subst_pw (sh 5)). var_solv.
+  rewrite - (subst_nat (sh 4)). var_solv. Qed. 
+
+  Hint Resolve uworld10 uworld32 uworld21.
+
+  Lemma store_type: forall W G,
+    (tr G (oof W world)) -> tr G (oof (store W) U0).
+Admitted.
+Hint Resolve store_type.
