help.v
@@ -1,3 +1,4 @@
+(*Shallow embedding of simple constructs from the monadic language into the store-passing logic*)
 
 From Coq Require Import Lists.List.
 From istari Require Import Tactics Sequence source subst_src rules_src.
@@ -5,7 +6,21 @@ From istari Require Import basic_types Syntax Subst SimpSub Promote Hygiene
      ContextHygiene Equivalence Rules Defined.
 
 
-(*he has arrow, you could be using arrow instead of pi if it makes it easier*)
+
+(*small abbreviations that will help us later*)
+Definition app3 w i u l : term False :=
+ app (app (app w i) u) l.
+
+(*quickly access the nth element of the big tuple in the comp type*)
+Definition picomp1 (M: term False) := ppi1 M.
+Definition picomp2 (M: term False) := ppi1 (ppi1 (ppi2 M) ). 
+Definition picomp3 (M: term False) := ppi2 (ppi1 (ppi2 M)). 
+Definition picomp4 (M: term False) := ppi2 (ppi2 M).
+(********************************************)
+
+
+
+(*useful types*)
 
 Definition plus L R : (term False) := sigma booltp (bite (var 0) (subst (sh 1) L)
                                            (subst (sh 1) R) ).
@@ -14,12 +29,14 @@ Definition inr R: term False := ppair bfalse R.
 
 Definition opt w: term False := sigma booltp (bite (var 0) w unittp).
 
-(*recursion*)
+Definition laters A : term False := rec (plus (shift 1 A) (fut (var 0))).
+(*notice similarity w type of nat in logic*)
+(********************************************)
 
-Definition combt A: (term False) := rec (
-                                    pi (fut (var 0)) (subst (sh 1) A)).
-(*probably have to shift A cuz its going under a binder*)
 
+(*useful terms*)
+
+(*Unguarded recursion*)
 Definition Yc: (term False) := lam ((*f := 0*)
                    app
                      (lam ( (*f := 1, x := 0*)
@@ -38,9 +55,7 @@ Definition Yc: (term False) := lam ((*f := 0*)
                 ))
 ).
 
-Definition laters A : term False := rec (plus (shift 1 A)  (fut (var 0))).
-  (*notice similarity w type of nat*)
-
+(*Computation monad*)
 Definition ret: term False := lam (inl (var 0)).
 
 Definition ret_t x := app ret x.
@@ -60,15 +75,8 @@ Definition bind : term False := app Yc
         ))).
 
 Definition make_bind E1 E2 := app (app bind E1) E2.
-(*worlds*)
 
-
-Definition preworld: (term False) := rec 
-                                   (arrow nattp (karrow (fut (var 0)) (arrow (fut nattp) U0))).
-
-Definition world: (term False) := sigma preworld nattp.
-
-Definition len w: (term False) := ppi2 w.
+(*arithmetic*)
 
 Definition if_z (n: term False): (term False) := ppi1 n.
 
@@ -100,16 +108,23 @@ Definition minusbc: (term False) := lam
                                                      (n)
                                                     (app (app f n) (app (ppi2 m) triv))
                                                   ))).
- Definition plus_n: (term False) := app theta plusbc.
+Definition plus_n: (term False) := app theta plusbc.
 
 Definition lt_b m n := if_z (app (app minus m) (nsucc n)).
 
-(*uses default value of w2*)
+(*worlds*)
 
-(*Definition cons w1 x :=
-  pend w1 (ppair (lam (let n := var 0 in bite (if_z n) x default_f)) one).*)
+Definition preworld: (term False) := rec 
+                                   (arrow nattp (karrow (fut (var 0)) (arrow (fut nattp) U0))).
 
-Definition cons_w w1 x :=
+Definition world: (term False) := sigma preworld nattp.
+
+Definition len w: (term False) := ppi2 w.
+
+Definition nth w n: term False := app (ppi1 w) n.
+
+(*default value after s(len w1) is x*)
+Definition cons_w x w1 :=
   ppair (lam ( (*n := 0*)
              let n := var 0 in
              bite (lt_b n (len w1))
@@ -117,19 +132,6 @@ Definition cons_w w1 x :=
                   x
         ))
         (nsucc (len w1)).
-(*default value after s(len w1) is x*
-ie uses default value of w2*)
-
-(*start here*)
-
-
-Definition app3 w i u l : term False :=
- app (app (app w i) u) l.
-
-Definition picomp1 (M: term False) := ppi1 M.
-Definition picomp2 (M: term False) := ppi1 (ppi1 (ppi2 M) ). 
-Definition picomp3 (M: term False) := ppi2 (ppi1 (ppi2 M)). 
-Definition picomp4 (M: term False) := ppi2 (ppi2 M). 
 
  Definition subseq: (term False) -> (term False) -> (term False) :=
    fun W1 => fun W2 =>
@@ -147,7 +149,7 @@ Definition picomp4 (M: term False) := ppi2 (ppi2 M).
                      (pi (nattp) (*u = 2, l = 1, i = 0*)(
                            pi (leq_t (var 0) (subst (sh 3) l1))
                               ( (*u = 3, l = 2, i = 1, m = 0*)
-                          eqtype (app3 (subst (sh 4) w1)                                         (var 1) (var 3) (var 2))
+                          eqtype (app3 (subst (sh 4) w1) (var 1) (var 3) (var 2))
                           (app3 (subst (sh 4) w2) (var 1) (var 3) (var 2))
                               )
                                                    )
@@ -155,78 +157,26 @@ Definition picomp4 (M: term False) := ppi2 (ppi2 M).
 
                  ))))) W1) W2.
 
- Definition nth w n: term False := app (ppi1 w) n.
-
  Definition make_subseq: term False := ppair triv (lam (lam (lam triv)) ).
 
+ (*transitivity of subseq*)
 
-Lemma subst_pw: forall s,
-    subst s preworld = preworld.
-intros. unfold preworld. unfold nattp. auto. Qed.
-Hint Rewrite subst_pw.
+ Lemma compose_sub_works : forall (M M' U1 U2 U3: term False) (G: context),
+                         tr G (oof M (subseq U2 U3))
+                         -> tr G (oof M' (subseq U1 U2))
+                         ->tr G (oof make_subseq 
+                                    (subseq U1 U3)).
+ Admitted.
 
+ (*need to do refl*)
 
-Lemma subst_world: forall s,
-    subst s world = world.
-intros. unfold world. unfold preworld. unfold nattp. auto. Qed.  
-Hint Rewrite subst_world.
-
-Lemma subst_nat: forall s,
-    @subst False s nattp = nattp.
-  intros. unfold nattp. auto. Qed.
-
-Hint Rewrite subst_nat.
-
-Lemma subst_nzero: forall s,
-    @subst False s nzero = nzero.
-  intros. unfold nzero. auto. Qed.
-Hint Rewrite subst_nzero.
-
-Lemma subst_leqtp: forall s,
-    @subst False s (leqtp) = leqtp.
-  intros. unfold leqtp. unfold wind. unfold theta.
-  repeat rewrite subst_app.
-  repeat rewrite subst_lam. simpsub. simpl.
-  repeat rewrite project_dot_succ.
-  rewrite project_dot_zero. auto. Qed.
-Hint Rewrite subst_leqtp.
-
-Lemma subst_bind: forall s m1 m2,
-    @subst False s (make_bind m1 m2) = make_bind (@subst False s m1) (@subst False s m2).
-  intros. auto. Qed.
+(*mysterious error Definition if_z (n: term False) := ppi1 n. *)
 
 
-Lemma subst_lttp: forall s,
-    @subst False s (lttp) = lttp.
-  intros. unfold lttp.
-  simpsub. rewrite subst_leqtp. unfold nsucc. simpsub. simpl.
-  rewrite subst_leqtp. auto. Qed.
-Hint Rewrite subst_leqtp.
 
-Lemma subst_leq: forall s n1 n2,
-    @subst False s (leq_t n1 n2) =  leq_t (subst s n1) (subst s n2).
-  intros. unfold leq_t.  repeat rewrite subst_app. rewrite subst_leqtp. auto. 
-Qed.
+(********************************************)
 
-Lemma subst_lt: forall s n1 n2,
-    subst s (app (app lttp n1) n2) = (app (app lttp (subst s n1)) (@subst False s n2)).
-  intros. repeat rewrite subst_app. rewrite subst_lttp. auto. Qed. 
-
-Lemma subst_subseq: forall W1 W2 s,
-       (subst s
-              (subseq W1 W2)) = subseq (subst s W1)
-                                       (subst s W2).
-  intros. unfold subseq. repeat rewrite subst_app. auto.
-Qed.
-
-
-Lemma subst_ret: forall s, subst s ret = ret.
-  intros. unfold ret. unfold inl. simpsub. auto. Qed.
-
-Lemma subst_ret_t: forall s m, subst s (ret_t m) = ret_t (subst s m).
-  intros. unfold ret_t. unfold ret. unfold inl. simpsub. auto. Qed.
-
-
+ (*memory store*)
 
  Definition getstore w v: (term False) := pi nattp ((*i = 0*)
                                            let i := var 0 in
@@ -241,87 +191,13 @@ Lemma subst_ret_t: forall s m, subst s (ret_t m) = ret_t (subst s m).
                                                     (subseq (var 1) (ppair (var 0) (shift 1 n) ))
                                                     (*u :=  var 1, m := var 0*)
                                                      (getstore (shift 2 w) (var 1))))) W.
-Lemma subst_U0: forall s,
-    (@subst False s (univ nzero)) = univ nzero.
-  auto. Qed.
 
 
-Lemma subst_store: forall W s, (subst s (store W)) = store (subst s W).
-  intros. unfold store. auto. Qed.
-Opaque store.
+(********************************************)
 
-Lemma subst_laters: forall s A, (subst s (laters A)) = (laters (subst s A)).
-  intros. unfold laters. unfold plus. rewrite subst_rec. rewrite subst_sigma.
-  rewrite subst_booltp. rewrite subst_bite. simpsub. simpl.
-  repeat rewrite <- subst_sh_shift. simpsub. auto. Qed.
+(*moving terms in a world to a future world*)
 
-Lemma subst_nth: forall s m1 m2, (subst s (nth m1 m2)) = (nth (subst s m1) (subst s m2)). intros. unfold nth. simpsub. auto. Qed.
-
-Lemma subst_make_subseq: forall s, (subst s make_subseq) = make_subseq.
-  intros. unfold make_subseq. simpsub. auto. Qed.
-
-Lemma subst_picomp1: forall s m, (subst s (picomp1 m)) = picomp1 (subst s m).
-  intros. unfold picomp1. simpsub. auto. Qed.
-
-Lemma subst_picomp2: forall s m, (subst s (picomp2 m)) = picomp2 (subst s m).
-  intros. unfold picomp2. simpsub. auto. Qed.
-
-Lemma subst_picomp3: forall s m, (subst s (picomp3 m)) = picomp3 (subst s m).
-  intros. unfold picomp3. simpsub. auto. Qed.
-
-Lemma subst_picomp4: forall s m, (subst s (picomp4 m)) = picomp4 (subst s m).
-  intros. unfold picomp4. simpsub. auto. Qed.
-
-Opaque laters.
-Opaque preworld.
-Opaque U0.
-Opaque subseq.
-Opaque leqtp.
-Opaque nzero.
-Opaque nattp.
-Opaque world.
-Opaque nth.
-
-Hint Rewrite subst_U0 subst_ret subst_ret_t: subst1.
-Hint Rewrite subst_subseq: subst1.
-Hint Rewrite subst_leq: subst1.
-Hint Rewrite subst_leqtp: subst1.
-Hint Rewrite subst_lttp: subst1.
-Hint Rewrite subst_lt: subst1.
-Hint Rewrite subst_nzero: subst1.
-Hint Rewrite subst_nat: subst1.
-Hint Rewrite subst_world: subst1.
-Hint Rewrite subst_pw: subst1.
-Hint Rewrite subst_world: subst1.
-Hint Rewrite subst_nth: subst1.
-Hint Rewrite subst_store: subst1.
-Hint Rewrite subst_laters
-subst_picomp1 subst_picomp2 subst_picomp4
-     subst_picomp3 subst_make_subseq: subst1.
-
-Ltac simpsub1 :=
-  autorewrite with subst1.
-
-
-
-
- (*M o M'*)
-
- Lemma compose_sub_works : forall (M M' U1 U2 U3: term False) (G: context),
-                         tr G (oof M (subseq U2 U3))
-                         -> tr G (oof M' (subseq U1 U2))
-                         ->tr G (oof make_subseq 
-                                    (subseq U1 U3)).
-Admitted.
-
- (*getstore w v = *(w/v)*)
-
- (*nats*)
-(*mysterious error Definition if_z (n: term False) := ppi1 n. *)
-
-
-
-(*start here get rid of vacuous cases w program module*)
+ (*start here get rid of vacuous cases w program module*)
  Definition move (A: source.term): term False :=
    match A with
      nattp_m => lam (lam (var 1))
@@ -360,25 +236,21 @@ end.
  Lemma subst_move: forall A s, (subst s (move A)) = move A.
    intros. induction A; simpsub; simpl; auto. Qed.
 
-
- (* for (var i): B in [n .. |G| + n],
-substitutes (move_B m i) in for i while leaving all other variables untouched
-
- in for nth variable of m while leaving all other vars untouched*)
- (*recursion will be to generate a substitution
-  that dots all of them on top of a shift |Gamma| *)
- Fixpoint sub_4_moveG (G: source.context) (m: term False) (n: nat (*starting variable*)) :=
+ (*moving all variables specified by G to a future world*)
+ (*n keeps track of index at which G starts*)
+ (* for (var i): B in G, (sub_4_moveG G m n) substitutes
+(move_B m (var (i + n))) in for (var (i + n)) while leaving all other variables untouched *)
+ Fixpoint sub_4_moveG (G: source.context) (m: term False) (n: nat) :=
  under n (match G with
    nil => id
           | b :: bs => dot (move_app b m (var 0)) (sub_4_moveG bs m (n + 1))
        end
 ).
 
- (*n is the counter *)
+ (*n keeps track of starting index*)
  Fixpoint move_gamma (G: source.context) (m: term False) (n: nat) :=
    subst (sub_4_moveG G m n).
 
-Opaque app.
 (*Lemma aaa: (move_gamma (cons nattp_m (cons unittp_m nil)) triv 1) (var 1) = unittp.
   simpl. simpsub. unfold move_app. simpsub. rewrite subst_move. unfold move. simpl.
   simpsub. simpl.
@@ -409,3 +281,6 @@ simpl. simpsub. simpl.*)
                        (subst (under 1 (dot (var 1) (dot (var 0) (sh 2)))) t) =
                             t.
   intros. simpsub. ring.*)
+
+
+Opaque laters preworld U0 subseq leqtp nzero nattp world nth.
