lemmas0.v
@@ -1,0 +1,17 @@
+Require Import Program.Equality Ring Lia Omega.
+From mathcomp Require Import ssreflect ssrfun ssrbool seq eqtype ssrnat.
+(*trivial small lemmas*)
+Lemma hseq2: forall (T: Type) (x y: T)
+                  (L: seq T), [:: x; y] ++ L=
+                 [:: x, y & L].
+intros. auto. Qed.
+
+  Lemma hseq3: forall (T: Type) (x y z: T)
+                  (L: seq T), [:: x; y; z] ++ L=
+                 [:: x, y, z & L].
+intros. auto. Qed.
+
+Lemma hseq4: forall (T: Type) (x y z a: T)
+                  (L: seq T), [:: x; y; z; a] ++ L=
+                 [:: x, y, z, a & L].
+intros. auto. Qed.
