subst_help.v
@@ -1,11 +1,10 @@
 From Coq.Lists Require Import List.
 From mathcomp Require Import ssreflect ssrfun ssrbool seq eqtype ssrnat.
-From istari Require Import source subst_src rules_src help.
+From istari Require Import source subst_src rules_src help subst_help0.
 From istari Require Import Sigma Tactics
      Syntax Subst SimpSub Promote Hygiene
      ContextHygiene Equivalence Rules Defined.
 
-(*basic substitution stuff*)
 
 Lemma eqsub_project : forall s s',
   (forall i,
